\documentclass{article}
\begin{document}
\noindent A simple \textbf{induction}:\\
$f(a^mb^n)$ = $a^{min(n, m)}b^{|m - n|}c^{min(n, m)}$\\
$f(a^xb^yc^k)$ = $b^{x+y}a^k$\\
$f(a^k)$ = $a^k$\\
A simple \textbf{series}:\\
$U_0  = m, V_0 = n$\\
$U_n = |U_{n-1} - V_{n-1}|, V_n = min(U_{n-1}, V_{n-1})$\\
$ \forall n \geq gcd(m, n), U_n = 0$\\\\
The \textbf{algorithm}:\\
\textbf{Input}: $a^mb^n$\\
1- Remove an 'a' an a 'b', otherwise (no a, no b or both) goto 3\\
2- Add 'c', goto 1\\
3- Switch all 'a' to 'b'\\
4- Switch all 'c' to 'a'\\
5- If there is 'b', goto 1, otherwise halt\\
\textbf{Output}: $a^x = a^{gcd(m, n)}$\\

\textbf{An explanation}:\\
The main idea is to continuously substruct n from m to get
a 'remainder' $|m - n|$ 'b' and  'quotient'  min(n, m)  'a'
until we get no more 'b' (remainder is 0) at step 4, therfore
$a^x = a^{gcd(n, m)}$\\


 \noindent A sample running:\\
aaaaaabbbbbbbbbb\\
aaaaabbbbbbbbb\\
aaaaabbbbbbbbbc\\
aaaabbbbbbbbc\\
aaaabbbbbbbbcc\\
aaabbbbbbbcc\\
aaabbbbbbbccc\\
aabbbbbbccc\\
aabbbbbbcccc\\
abbbbbcccc\\
abbbbbccccc\\
bbbbccccc\\
bbbbcccccc\\
bbbbaaaaaa\\
bbbaaaaa\\
bbbaaaaac\\
bbaaaac\\
bbaaaacc\\
baaacc\\
baaaccc\\
aaccc\\
aacccc\\
bbcccc\\
bbaaaa\\
baaa\\
baaac\\
aac\\
aacc\\
bbaa\\
ba\\
bac\\
cc\\
aa\\
HALT\\
GCD(14, 6) = 2
\end{document}
